VERIFIED

```latex
\section*{Question 12: Trigonometric Sums and Riemann Sums}

\subsection*{Part (a): Trigonometric Identity and Sum Formula}

\textbf{Step 1: Derive the product-to-sum identity.}

Starting with the addition formulas:
\begin{align}
\cos(a + b) &= \cos a \cos b - \sin a \sin b \\
\cos(a - b) &= \cos a \cos b + \sin a \sin b
\end{align}

Subtracting equation (1) from equation (2):
\begin{align}
\cos(a - b) - \cos(a + b) &= 2\sin a \sin b
\end{align}

Therefore:
\begin{equation}
\cos(a + b) - \cos(a - b) = -2\sin a \sin b
\end{equation}

\textbf{Step 2: Apply to the specific case.}

Let $a = jt$ and $b = \frac{t}{2}$. Then:
\begin{align}
a + b &= jt + \frac{t}{2} = \left(j + \frac{1}{2}\right)t \\
a - b &= jt - \frac{t}{2} = \left(j - \frac{1}{2}\right)t
\end{align}

Substituting into equation (4):
\[
\boxed{\cos\left(\left(j + \frac{1}{2}\right)t\right) - \cos\left(\left(j - \frac{1}{2}\right)t\right) = -2\sin\left(\frac{t}{2}\right)\sin(jt)}
\]

\textbf{Step 3: Derive the sum formula using telescoping.}

Rearranging the identity:
\[
\sin(jt) = \frac{\cos\left(\left(j - \frac{1}{2}\right)t\right) - \cos\left(\left(j + \frac{1}{2}\right)t\right)}{2\sin\left(\frac{t}{2}\right)}
\]

This is valid when $\sin\left(\frac{t}{2}\right) \neq 0$, i.e., when $\frac{t}{2\pi}$ is not an integer.

Summing from $j = 1$ to $n$:
\[
\sum_{j=1}^{n} \sin(jt) = \frac{1}{2\sin\left(\frac{t}{2}\right)} \sum_{j=1}^{n} \left[\cos\left(\left(j - \frac{1}{2}\right)t\right) - \cos\left(\left(j + \frac{1}{2}\right)t\right)\right]
\]

The sum telescopes:
\begin{align*}
&\sum_{j=1}^{n} \left[\cos\left(\left(j - \frac{1}{2}\right)t\right) - \cos\left(\left(j + \frac{1}{2}\right)t\right)\right] \\
&= \left[\cos\left(\frac{t}{2}\right) - \cos\left(\frac{3t}{2}\right)\right] + \left[\cos\left(\frac{3t}{2}\right) - \cos\left(\frac{5t}{2}\right)\right] + \cdots + \left[\cos\left(\left(n - \frac{1}{2}\right)t\right) - \cos\left(\left(n + \frac{1}{2}\right)t\right)\right] \\
&= \cos\left(\frac{t}{2}\right) - \cos\left(\left(n + \frac{1}{2}\right)t\right)
\end{align*}

Therefore:
\[
\boxed{\sum_{j=1}^{n} \sin(jt) = \frac{\cos\left(\frac{t}{2}\right) - \cos\left(\left(n + \frac{1}{2}\right)t\right)}{2\sin\left(\frac{t}{2}\right)}}
\]

\subsection*{Part (b): Evaluating the Integral via Riemann Sum}

\textbf{Step 1: Set up the Riemann sum.}

To evaluate $\displaystyle\int_0^b \sin x \, dx$ where $0 < b < \frac{\pi}{2}$, partition $[0, b]$ into $n$ equal subintervals.

Let $\Delta x = \frac{b}{n}$ and use right endpoints $x_j = j \cdot \frac{b}{n}$ for $j = 1, 2, \ldots, n$.

The Riemann sum is:
\[
R_n = \sum_{j=1}^{n} \sin(x_j) \cdot \Delta x = \sum_{j=1}^{n} \sin\left(\frac{jb}{n}\right) \cdot \frac{b}{n} = \frac{b}{n} \sum_{j=1}^{n} \sin\left(\frac{jb}{n}\right)
\]

\textbf{Step 2: Apply the sum formula from part (a).}

Let $t = \frac{b}{n}$. Since $0 < b < \frac{\pi}{2}$ and $n \geq 1$, we have $0 < t < \frac{\pi}{2}$, so $\frac{t}{2\pi}$ is not an integer.

By part (a):
\[
\sum_{j=1}^{n} \sin(jt) = \frac{\cos\left(\frac{t}{2}\right) - \cos\left(\left(n + \frac{1}{2}\right)t\right)}{2\sin\left(\frac{t}{2}\right)}
\]

With $t = \frac{b}{n}$:
\[
\sum_{j=1}^{n} \sin\left(\frac{jb}{n}\right) = \frac{\cos\left(\frac{b}{2n}\right) - \cos\left(\frac{(2n+1)b}{2n}\right)}{2\sin\left(\frac{b}{2n}\right)}
\]

Therefore:
\[
R_n = \frac{b}{n} \cdot \frac{\cos\left(\frac{b}{2n}\right) - \cos\left(b + \frac{b}{2n}\right)}{2\sin\left(\frac{b}{2n}\right)}
\]

\textbf{Step 3: Evaluate the limit as $n \to \infty$.}

Rewrite as:
\[
R_n = \frac{b}{2n\sin\left(\frac{b}{2n}\right)} \cdot \left[\cos\left(\frac{b}{2n}\right) - \cos\left(b + \frac{b}{2n}\right)\right]
\]

Let $u = \frac{b}{2n}$, so as $n \to \infty$, $u \to 0^+$.

\textbf{First factor:} Using $\lim_{u \to 0} \frac{\sin u}{u} = 1$:
\[
\lim_{n \to \infty} \frac{b}{2n\sin\left(\frac{b}{2n}\right)} = \lim_{u \to 0^+} \frac{u}{\sin u} = 1
\]

\textbf{Second factor:} As $n \to \infty$:
\[
\lim_{n \to \infty} \left[\cos\left(\frac{b}{2n}\right) - \cos\left(b + \frac{b}{2n}\right)\right] = \cos(0) - \cos(b) = 1 - \cos b
\]

\textbf{Step 4: Combine the limits.}

\[
\int_0^b \sin x \, dx = \lim_{n \to \infty} R_n = 1 \cdot (1 - \cos b) = 1 - \cos b
\]

\textbf{Verification:} By the Fundamental Theorem of Calculus:
\[
\int_0^b \sin x \, dx = [-\cos x]_0^b = -\cos b - (-\cos 0) = 1 - \cos b \quad \checkmark
\]

\[
\boxed{\int_0^b \sin x \, dx = 1 - \cos b}
\]
```
