```latex
\section*{Question 2: Derivatives and Antiderivatives}

Give the derivatives and antiderivatives of each of the following, where $c > 0$ is a constant.

\textbf{Useful Lemma:} First, let us prove that an antiderivative of $\ln(x)$ is $x\ln(x) - x$.

\textit{Proof:} We verify by differentiation:
\[\frac{d}{dx}\left(x\ln(x) - x\right) = \ln(x) + x \cdot \frac{1}{x} - 1 = \ln(x) + 1 - 1 = \ln(x) \quad \checkmark\]

\bigskip

\subsection*{(a) $c^{2x}$}

\textbf{Derivative:} Rewrite using exponential form: $c^{2x} = e^{2x\ln(c)}$

Using the chain rule:
\[\frac{d}{dx}\left(c^{2x}\right) = e^{2x\ln(c)} \cdot 2\ln(c) = \boxed{2\ln(c) \cdot c^{2x}}\]

\textbf{Antiderivative:} 
\[\int c^{2x}\,dx = \int e^{2x\ln(c)}\,dx = \frac{e^{2x\ln(c)}}{2\ln(c)} + C = \boxed{\frac{c^{2x}}{2\ln(c)} + C}\]

\bigskip

\subsection*{(b) $x^{2c}$}

\textbf{Derivative:} Using the power rule (since $2c$ is a constant):
\[\frac{d}{dx}\left(x^{2c}\right) = \boxed{2c \cdot x^{2c-1}}\]

\textbf{Antiderivative:} Using the power rule for integration:
\[\int x^{2c}\,dx = \frac{x^{2c+1}}{2c+1} + C = \boxed{\frac{x^{2c+1}}{2c+1} + C}\]

\bigskip

\subsection*{(c) $\sin(cx)$}

\textbf{Derivative:} Using the chain rule:
\[\frac{d}{dx}\left(\sin(cx)\right) = \cos(cx) \cdot c = \boxed{c\cos(cx)}\]

\textbf{Antiderivative:} 
\[\int \sin(cx)\,dx = -\frac{1}{c}\cos(cx) + C = \boxed{-\frac{\cos(cx)}{c} + C}\]

\bigskip

\subsection*{(d) $x\ln(cx^2)$}

\textbf{Derivative:} First simplify: $x\ln(cx^2) = x\ln(c) + 2x\ln(x)$

Using the product rule on $2x\ln(x)$:
\[\frac{d}{dx}\left(x\ln(c) + 2x\ln(x)\right) = \ln(c) + 2\left(\ln(x) + x \cdot \frac{1}{x}\right) = \ln(c) + 2\ln(x) + 2\]

This can also be written as:
\[\boxed{\ln(c) + 2\ln(x) + 2 = \ln(cx^2) + 2}\]

\textbf{Antiderivative:} Using the simplified form $x\ln(c) + 2x\ln(x)$:
\[\int \left(x\ln(c) + 2x\ln(x)\right)dx = \ln(c) \cdot \frac{x^2}{2} + 2\int x\ln(x)\,dx\]

For $\int x\ln(x)\,dx$, use integration by parts with $u = \ln(x)$, $dv = x\,dx$:
\[\int x\ln(x)\,dx = \frac{x^2}{2}\ln(x) - \int \frac{x^2}{2} \cdot \frac{1}{x}\,dx = \frac{x^2}{2}\ln(x) - \frac{x^2}{4}\]

Therefore:
\[\int x\ln(cx^2)\,dx = \frac{x^2\ln(c)}{2} + 2\left(\frac{x^2\ln(x)}{2} - \frac{x^2}{4}\right) = \frac{x^2\ln(c)}{2} + x^2\ln(x) - \frac{x^2}{2}\]

\[\boxed{\frac{x^2\ln(cx^2)}{2} - \frac{x^2}{2} + C = \frac{x^2}{2}\left(\ln(cx^2) - 1\right) + C}\]

\bigskip

\subsection*{(e) $e^{cx}$}

\textbf{Derivative:} Using the chain rule:
\[\frac{d}{dx}\left(e^{cx}\right) = e^{cx} \cdot c = \boxed{ce^{cx}}\]

\textbf{Antiderivative:} 
\[\int e^{cx}\,dx = \boxed{\frac{e^{cx}}{c} + C}\]
```
