```latex
\section*{Question 10: Second-Order Linear ODE}

Find the general solution of the differential equation:
\[
y'' - 2y' + y = e^{2x}
\]

\subsection*{Solution}

This is a second-order linear ODE with constant coefficients. We solve it by finding the homogeneous solution $y_h$ and a particular solution $y_p$.

\subsubsection*{Step 1: Solve the Homogeneous Equation}

Consider the homogeneous equation:
\[
y'' - 2y' + y = 0
\]

The characteristic equation is:
\[
r^2 - 2r + 1 = 0
\]

Factoring:
\[
(r - 1)^2 = 0
\]

This gives a repeated root $r = 1$ with multiplicity 2.

For a repeated root, the homogeneous solution is:
\[
y_h = C_1 e^x + C_2 x e^x
\]

\subsubsection*{Step 2: Find a Particular Solution}

Since the right-hand side is $e^{2x}$ and $r = 2$ is \textit{not} a root of the characteristic equation, we try a particular solution of the form:
\[
y_p = A e^{2x}
\]

Compute the derivatives:
\[
y_p' = 2A e^{2x}
\]
\[
y_p'' = 4A e^{2x}
\]

Substitute into the differential equation:
\[
y_p'' - 2y_p' + y_p = 4A e^{2x} - 2(2A e^{2x}) + A e^{2x}
\]
\[
= 4A e^{2x} - 4A e^{2x} + A e^{2x}
\]
\[
= A e^{2x}
\]

Setting this equal to $e^{2x}$:
\[
A e^{2x} = e^{2x}
\]

Therefore:
\[
A = 1
\]

The particular solution is:
\[
y_p = e^{2x}
\]

\subsubsection*{Step 3: Write the General Solution}

The general solution is:
\[
y = y_h + y_p
\]

\[
\boxed{y = C_1 e^x + C_2 x e^x + e^{2x}}
\]

where $C_1$ and $C_2$ are arbitrary constants.
```
